first try at proving 4.1. need better alpha equivalence

theories/Smallstep.v
@@ -24,154 +24,112 @@ Record config : Type := {
   cfg_stack : stack
 }.
 
+Open Scope string_scope.
+Reserved Notation "c1 s=> c2" (at level 70).
 Inductive step : config -> config -> Prop :=
   (** expr evaluation rules *)
 
   (* (e y) pushes y onto stack and evaluates e *)
   | StepApp1 : forall G e y St,
-    step {| cfg_heap := G;
-            cfg_ctrl := CtrlExpr (EApp e (EVar y));
-            cfg_stack := St |}
-          {| cfg_heap := G;
-            cfg_ctrl := CtrlExpr e;
-            cfg_stack := KArg y :: St |}
+      {| cfg_heap := G; cfg_ctrl := CtrlExpr (EApp e (EVar y)); cfg_stack := St |}
+      s=>
+      {| cfg_heap := G; cfg_ctrl := CtrlExpr e; cfg_stack := KArg y :: St |}
 
   (* lambda with arity > 0 consumes argument from stack *)
   | StepApp2 : forall G m y St n,
       matching_arity m = Some (S n) ->
-      step {| cfg_heap := G;
-              cfg_ctrl := CtrlExpr (ELam m);
-              cfg_stack := KArg y :: St |}
-           {| cfg_heap := G;
-              cfg_ctrl := CtrlExpr (ELam (MSupply (EVar y) m));
-              cfg_stack := St |}
+      {| cfg_heap := G; cfg_ctrl := CtrlExpr (ELam m); cfg_stack := KArg y :: St |}
+      s=>
+      {| cfg_heap := G; cfg_ctrl := CtrlExpr (ELam (MSupply (EVar y) m)); cfg_stack := St |}
 
   (* saturated matching (arity 0) switches to matching evaluation *)
   | StepSat : forall G m St,
       matching_arity m = Some 0 ->
-      step {| cfg_heap := G;
-              cfg_ctrl := CtrlExpr (ELam m);
-              cfg_stack := St |}
-           {| cfg_heap := G;
-              cfg_ctrl := CtrlMatch [] m;
-              cfg_stack := KEnd :: St |}
+      {| cfg_heap := G; cfg_ctrl := CtrlExpr (ELam m); cfg_stack := St |}
+      s=>
+      {| cfg_heap := G; cfg_ctrl := CtrlMatch [] m; cfg_stack := KEnd :: St |}
 
   (* lookup variable in heap and mark for update *)
   | StepVar : forall G y e St,
       heap_lookup G y = Some e ->
-      step {| cfg_heap := G;
-              cfg_ctrl := CtrlExpr (EVar y);
-              cfg_stack := St |}
-           {| cfg_heap := heap_remove G y;
-              cfg_ctrl := CtrlExpr e;
-              cfg_stack := KUpdate y :: St |}
+      {| cfg_heap := G; cfg_ctrl := CtrlExpr (EVar y); cfg_stack := St |}
+      s=>
+      {| cfg_heap := heap_remove G y; cfg_ctrl := CtrlExpr e; cfg_stack := KUpdate y :: St |}
 
   (* update heap with whnf *)
   | StepUpdate : forall G y w St,
       whnf w ->
-      step {| cfg_heap := G;
-              cfg_ctrl := CtrlExpr w;
-              cfg_stack := KUpdate y :: St |}
-           {| cfg_heap := heap_update G y w;
-              cfg_ctrl := CtrlExpr w;
-              cfg_stack := St |}
+      {| cfg_heap := G; cfg_ctrl := CtrlExpr w; cfg_stack := KUpdate y :: St |}
+      s=>
+      {| cfg_heap := heap_update G y w; cfg_ctrl := CtrlExpr w; cfg_stack := St |}
 
   (** matching evaluation rules *)
 
   (* return with non-empty argument stack applies arguments *)
   | StepReturn1A : forall G A e St,
       A <> [] ->
-      step {| cfg_heap := G;
-              cfg_ctrl := CtrlMatch A (MReturn e);
-              cfg_stack := St |}
-           {| cfg_heap := G;
-              cfg_ctrl := CtrlMatch [] (MReturn (apply_args A e));
-              cfg_stack := St |}
+      {| cfg_heap := G; cfg_ctrl := CtrlMatch A (MReturn e); cfg_stack := St |}
+      s=>
+      {| cfg_heap := G; cfg_ctrl := CtrlMatch [] (MReturn (apply_args A e)); cfg_stack := St |}
 
   (* return with empty args and $ mark evaluates expression *)
   | StepReturn1B : forall G e St,
-      step {| cfg_heap := G;
-              cfg_ctrl := CtrlMatch [] (MReturn e);
-              cfg_stack := KEnd :: St |}
-           {| cfg_heap := G;
-              cfg_ctrl := CtrlExpr e;
-              cfg_stack := St |}
+      {| cfg_heap := G; cfg_ctrl := CtrlMatch [] (MReturn e); cfg_stack := KEnd :: St |}
+      s=>
+      {| cfg_heap := G; cfg_ctrl := CtrlExpr e; cfg_stack := St |}
 
   (* Return2: return with empty args and alternative on stack discards alternative *)
   | StepReturn2 : forall G e A' m St,
-      step {| cfg_heap := G;
-              cfg_ctrl := CtrlMatch [] (MReturn e);
-              cfg_stack := KAlt A' m :: St |}
-           {| cfg_heap := G;
-              cfg_ctrl := CtrlMatch [] (MReturn e);
-              cfg_stack := St |}
+      {| cfg_heap := G; cfg_ctrl := CtrlMatch [] (MReturn e); cfg_stack := KAlt A' m :: St |}
+      s=>
+      {| cfg_heap := G; cfg_ctrl := CtrlMatch [] (MReturn e); cfg_stack := St |}
 
   (* variable pattern performs substitution *)
   | StepBind : forall G y A x m St,
-      step {| cfg_heap := G;
-              cfg_ctrl := CtrlMatch (y :: A) (MMatch (PVar x) m);
-              cfg_stack := St |}
-           {| cfg_heap := G;
-              cfg_ctrl := CtrlMatch A (subst_matching m y x);
-              cfg_stack := St |}
+      {| cfg_heap := G; cfg_ctrl := CtrlMatch (y :: A) (MMatch (PVar x) m); cfg_stack := St |}
+      s=>
+      {| cfg_heap := G; cfg_ctrl := CtrlMatch A (subst_matching m y x); cfg_stack := St |}
 
   (* constructor pattern switches to expression evaluation *)
   | StepCons1 : forall G y A c ps m St,
-      step {| cfg_heap := G;
-              cfg_ctrl := CtrlMatch (y :: A) (MMatch (PCons c ps) m);
-              cfg_stack := St |}
-           {| cfg_heap := G;
-              cfg_ctrl := CtrlExpr (EVar y);
-              cfg_stack := KPat A c ps m :: St |}
+      {| cfg_heap := G; cfg_ctrl := CtrlMatch (y :: A) (MMatch (PCons c ps) m); cfg_stack := St |}
+      s=>
+      {| cfg_heap := G; cfg_ctrl := CtrlExpr (EVar y); cfg_stack := KPat A c ps m :: St |}
 
   (* successful constructor match decomposes into nested matches *)
   | StepCons2 : forall G c args A ps m St,
       length args = length ps ->
-      step {| cfg_heap := G;
-              cfg_ctrl := CtrlExpr (ECons c (map EVar args));
-              cfg_stack := KPat A c ps m :: St |}
-           {| cfg_heap := G;
-              cfg_ctrl := CtrlMatch A (build_nested_matches args ps m);
-              cfg_stack := St |}
+      {| cfg_heap := G; cfg_ctrl := CtrlExpr (ECons c (map EVar args)); cfg_stack := KPat A c ps m :: St |}
+      s=>
+      {| cfg_heap := G; cfg_ctrl := CtrlMatch A (build_nested_matches args ps m); cfg_stack := St |}
 
   (* constructor mismatch leads to failure *)
   | StepFail : forall G c c' args A ps m St,
       c <> c' ->
-      step {| cfg_heap := G;
-              cfg_ctrl := CtrlExpr (ECons c' args);
-              cfg_stack := KPat A c ps m :: St |}
-           {| cfg_heap := G;
-              cfg_ctrl := CtrlMatch [] MFail;
-              cfg_stack := St |}
+      {| cfg_heap := G; cfg_ctrl := CtrlExpr (ECons c' args); cfg_stack := KPat A c ps m :: St |}
+      s=>
+      {| cfg_heap := G; cfg_ctrl := CtrlMatch [] MFail; cfg_stack := St |}
 
   (* argument supply pushes argument onto local stack *)
   | StepArg : forall G A y m St,
-      step {| cfg_heap := G;
-              cfg_ctrl := CtrlMatch A (MSupply (EVar y) m);
-              cfg_stack := St |}
-           {| cfg_heap := G;
-              cfg_ctrl := CtrlMatch (y :: A) m;
-              cfg_stack := St |}
+      {| cfg_heap := G; cfg_ctrl := CtrlMatch A (MSupply (EVar y) m); cfg_stack := St |}
+      s=>
+      {| cfg_heap := G; cfg_ctrl := CtrlMatch (y :: A) m; cfg_stack := St |}
 
   (* alternative pushes second branch onto stack *)
   | StepAlt1 : forall G A m1 m2 St,
-      step {| cfg_heap := G;
-              cfg_ctrl := CtrlMatch A (MAlt m1 m2);
-              cfg_stack := St |}
-           {| cfg_heap := G;
-              cfg_ctrl := CtrlMatch A m1;
-              cfg_stack := KAlt A m2 :: St |}
+      {| cfg_heap := G; cfg_ctrl := CtrlMatch A (MAlt m1 m2); cfg_stack := St |}
+      s=>
+      {| cfg_heap := G; cfg_ctrl := CtrlMatch A m1; cfg_stack := KAlt A m2 :: St |}
 
   (* failure pops alternative from stack *)
   | StepAlt2 : forall G A' A m St,
-      step {| cfg_heap := G;
-              cfg_ctrl := CtrlMatch A' MFail;
-              cfg_stack := KAlt A m :: St |}
-           {| cfg_heap := G;
-              cfg_ctrl := CtrlMatch A m;
-              cfg_stack := St |}
+      {| cfg_heap := G; cfg_ctrl := CtrlMatch A' MFail; cfg_stack := KAlt A m :: St |}
+      s=>
+      {| cfg_heap := G; cfg_ctrl := CtrlMatch A m; cfg_stack := St |}
 
   (* allocate bindings in heap with fresh variables *)
+
   (*| StepWhere : forall G A m binds St ys renamed_binds renamed_m,*)
   (*    length ys = length binds ->*)
   (*    (* ys are fresh *)*)
@@ -179,25 +137,34 @@ Inductive step : config -> config -> Prop :=
   (*    (* perform renaming *)*)
   (*    renamed_binds = rename_bindings binds ys ->*)
   (*    renamed_m = rename_matching m ys binds ->*)
-  (*    step {| cfg_heap := G;*)
-  (*            cfg_ctrl := CtrlMatch A (MWhere m binds);*)
-  (*            cfg_stack := St |}*)
-  (*         {| cfg_heap := allocate_bindings G renamed_binds;*)
-  (*            cfg_ctrl := CtrlMatch A renamed_m;*)
-  (*            cfg_stack := St |}*)
-.
+  (*    {| cfg_heap := G; cfg_ctrl := CtrlMatch A (MWhere m binds); cfg_stack := St |}*)
+  (*    s=> *)
+  (*    {| cfg_heap := allocate_bindings G renamed_binds; cfg_ctrl := CtrlMatch A renamed_m; cfg_stack := St |}*)
+
+  (* avoid alpha convergence *)
+  | StepWhere : forall G A m binds St,
+      let avoid := map fst (StringMap.elements G) in
+      let ys := generate_fresh_vars "y" (length binds) avoid in
+      {| cfg_heap := G; cfg_ctrl := CtrlMatch A (MWhere m binds); cfg_stack := St |}
+      s=>
+      {| cfg_heap := allocate_bindings G (rename_bindings binds ys);
+        cfg_ctrl := CtrlMatch A (rename_matching m ys binds);
+        cfg_stack := St |}
+
+where "c1 s=> c2" := (step c1 c2).
+Close Scope string_scope.
 
 (* refl and transitive closure of step *)
+
+Reserved Notation "c1 s=>* c2" (at level 40).
 Inductive step_star : config -> config -> Prop :=
   | step_refl : forall c,
-      step_star c c
+      c s=>* c
   | step_trans : forall c1 c2 c3,
-      step c1 c2 ->
-      step_star c2 c3 ->
-      step_star c1 c3.
-
-Notation "c1 s=> c2" := (step c1 c2) (at level 70).
-Notation "c1 s=>* c2" := (step_star c1 c2) (at level 70).
+      c1 s=> c2 ->
+      c2 s=>* c3 ->
+      c1 s=>* c3
+where "c1 s=>* c2" := (step_star c1 c2).
 
 Lemma step_star_one : forall c1 c2,
   c1 s=> c2 -> c1 s=>* c2.
@@ -278,8 +245,34 @@ Proof.
   (* others solved by proving that the whnf is impossible *)
   try solve_determinism_small.
 
-  inversion H8; subst.
-  apply map_EVar_inj in H3; subst.
-  inversion H9; subst.
-  reflexivity.
+  - inversion H8; subst.
+    apply map_EVar_inj in H3; subst.
+    inversion H9; subst.
+    reflexivity.
+  - inversion H7; subst.
+    assert (ys = ys0). { reflexivity. }
+    rewrite H.
+    reflexivity.
 Qed.
+
+Lemma step_star_step : forall c1 c2 c3,
+  c1 s=>* c2 ->
+  c2 s=> c3 ->
+  c1 s=>* c3.
+Proof.
+  intros c1 c2 c3 Hstar Hstep.
+  induction Hstar.
+  - eapply step_trans; eauto. constructor.
+  - eapply step_trans; eauto.
+Qed.
+
+(*Lemma step_star_under_continuation : forall G A m D mu St k,*)
+(*  {| cfg_heap := G; cfg_ctrl := CtrlMatch A m; cfg_stack := St |} s=>**)
+(*  {| cfg_heap := D; cfg_ctrl := CtrlMatch [] mu; cfg_stack := St |} ->*)
+(**)
+(*  {| cfg_heap := G; cfg_ctrl := CtrlMatch A m; cfg_stack := k :: St |} s=>**)
+(*  {| cfg_heap := D; cfg_ctrl := CtrlMatch [] mu; cfg_stack := k :: St |}.*)
+(*Proof.*)
+(*  intros G A m D mu St k Heval.*)
+(*  induction Heval.*)
+
