theories/Semantics_equiv.v
@@ -1,0 +1,167 @@
+From Coq Require Import String Arith List.
+From Coq Require Import FMaps FSets.
+From Haskelite Require Import Expr Common Bigstep Smallstep.
+Import ListNotations.
+
+Lemma eval_expr_produces_whnf : forall G L e D w,
+  eval_expr G L e D w -> whnf w.
+Proof.
+  intros. induction H; assumption.
+Qed.
+
+Lemma whnf_lambda_arity : forall m,
+  whnf (ELam m) ->
+  exists n, matching_arity m = Some (S n).
+Proof.
+  intros m H.
+  inversion H; subst.
+  exists n. assumption.
+Qed.
+
+Lemma eval_expr_lambda_arity : forall G L e D m,
+  eval_expr G L e D (ELam m) ->
+  exists n, matching_arity m = Some (S n).
+Proof.
+  intros G L e D m H.
+  apply whnf_lambda_arity.
+  eapply eval_expr_produces_whnf.
+  eassumption.
+Qed.
+
+(* theorem 4.1 *)
+Theorem big_step_impl_small_step :
+  (forall G L e D w,
+    eval_expr G L e D w ->
+    forall St, {| cfg_heap := G; cfg_ctrl := CtrlExpr e; cfg_stack := St |} s=>*
+               {| cfg_heap := D; cfg_ctrl := CtrlExpr w; cfg_stack := St |})
+  /\
+  (forall G L A m D u,
+    eval_matching G L A m D u ->
+    forall St, {| cfg_heap := G; cfg_ctrl := CtrlMatch A m; cfg_stack := St |} s=>*
+               {| cfg_heap := D; cfg_ctrl := CtrlMatch []
+                                  (match u with MRReturn e => MReturn e | MRFail => MFail end); 
+                  cfg_stack := St |}).
+Proof.
+  apply eval_ind.
+  - intros G L w Hwhnf St.
+    constructor.
+  - intros G L m e D O w Harity Hmatch IHmatch Heval IHeval St.
+    eapply step_star_trans.
+    + eapply step_trans.
+      * apply StepSat. eassumption.
+      * apply step_refl.
+    + eapply step_star_trans.
+      * apply IHmatch.
+      * eapply step_star_trans.
+        ** eapply step_trans.
+           -- apply StepReturn1B.
+           -- apply step_refl.
+        ** apply IHeval.
+
+  - intros G L y e D w Hheap Hin Heval IHexpr St.
+    eapply step_star_trans.
+    + eapply step_trans.
+      * apply StepVar. eassumption.
+      * apply step_refl.
+    + eapply step_star_trans.
+      * apply IHexpr.
+      * eapply step_trans.
+        ** apply StepUpdate. eapply eval_expr_produces_whnf. eassumption.
+        ** apply step_refl.
+
+  - intros G L e1 e2 m D O w x Hexpr1 IHexpr Hvar Hexpr2 IHexpr2 St.
+    subst e2.
+    destruct (eval_expr_lambda_arity _ _ _ _ _ Hexpr1) as [n Harity].
+    eapply step_star_trans.
+    + eapply step_trans.
+      * apply StepApp1.
+      * apply step_refl.
+    + eapply step_star_trans.
+      * apply IHexpr.
+      * eapply step_star_trans.
+        ** eapply step_trans.
+           ++ eapply StepApp2. eassumption.
+           ++ apply step_refl.
+        ** apply IHexpr2.
+
+  - intros G L A e St.
+    destruct A as [| y A'].
+    + simpl. apply step_refl.
+    + eapply step_star_trans.
+      * eapply step_trans.
+        ** apply StepReturn1A. discriminate.
+        ** apply step_refl.
+      * apply step_refl.
+
+  - intros G L st. apply step_refl.
+
+  - intros G L A x m D u _ IHmatch St.
+    eapply step_star_trans.
+    + eapply step_trans.
+      * apply StepArg.
+      * apply step_refl.
+    + apply IHmatch.
+
+  - intros G L A x y m D u _ IHmatch St.
+    eapply step_star_trans.
+    + eapply step_trans.
+      * apply StepBind.
+      * apply step_refl.
+    + apply IHmatch.
+
+  - intros G L A x c ps m args D O u Hexpr IHexpr Hlen Hmatching IHmatching St.
+    eapply step_star_trans.
+    + eapply step_trans.
+      * apply StepCons1.
+      * apply step_refl.
+    + eapply step_star_trans.
+      * apply IHexpr.
+      * eapply step_star_trans.
+        ** eapply step_trans.
+           ++ apply StepCons2. symmetry. assumption.
+           ++ apply step_refl.
+        ** apply IHmatching.
+
+  - intros G L A x c c' ps m args D Hexpr IHexpr Heqc St.
+    eapply step_star_trans.
+    + eapply step_trans.
+      * apply StepCons1.
+      * apply step_refl.
+    + eapply step_star_trans.
+      * apply IHexpr.
+      * eapply step_trans.
+        ** apply StepFail. assumption.
+        ** apply step_refl.
+
+  - intros G L A m1 m2 e D Hmatching IHmatch St.
+    eapply step_star_trans.
+    + eapply step_trans.
+      * apply StepAlt1.
+      * apply step_refl.
+    + eapply step_star_trans.
+      * apply IHmatch.
+      * eapply step_trans.
+        ** apply StepReturn2.
+        ** apply step_refl.
+
+  - intros G L A m1 m2 D O u Hmatching1 IHmatch1 Hmatching2 IHmatch2 St.
+    eapply step_star_trans.
+    + eapply step_trans.
+      * apply StepAlt1.
+      * apply step_refl.
+    + eapply step_star_trans.
+      * apply IHmatch1.
+      * eapply step_star_trans.
+        ** constructor.
+        ** eapply step_trans.
+           ++ constructor.
+           ++  apply IHmatch2.
+
+  - intros G L A m binds D u avoid ys Hmatching IHmatch St.
+    eapply step_star_trans.
+    + constructor.
+    + eapply step_trans.
+      * constructor.
+      * admit. (* need better alternative, maybe add an alpha equivalence relation and prove to aeq? *)
+Admitted.
+
